lang/let_lift.v
@@ -1,0 +1,72 @@
+From Ltac2 Require Import Ltac2.
+Module UConstr := Constr.Unsafe.
+
+Local Ltac2 Type collect_consts_state := {
+  mutable lets : (ident option * constr * Constr.Binder.relevance * constr) list;
+  mutable m : (constant, int) FMap.t;
+  mutable n : int;
+}.
+Ltac2 collect_consts (filter : constant -> instance -> bool) (e : constr) :=
+  let st := { lets := []; m := FMap.empty FSet.Tags.constant_tag; n := 0 } in
+  let rec collect (e : constr) : unit :=
+    match UConstr.kind e with
+    | UConstr.Constant c i =>
+      if FMap.mem c (st.(m)) then () else
+      if Bool.neg (filter c i) then () else (
+      match Control.case (fun () => Std.eval_cbv { RedFlags.none with Std.rConst := [Std.ConstRef c]} e) with
+      | Err _ => () | Val (body, _) => 
+      if Constr.equal e body then () else (
+      st.(m) := FMap.add c (-1) (st.(m));
+      let rec last l := match l with [] => None | x :: [] => (Some x) | x :: xs => last xs end in
+      let name := last (Env.path (Std.ConstRef c)) in
+      let typ := Constr.type e in
+      collect typ; collect body;
+      let relevance := if Constr.equal (Std.eval_hnf (Constr.type typ)) 'SProp then Constr.Binder.Irrelevant else Constr.Binder.Relevant in (* Question: is this line always correct? *)
+      st.(lets) := ((name, typ, relevance, body) :: st.(lets));
+      st.(m) := FMap.add c (st.(n)) (st.(m));
+      st.(n) := Int.add (st.(n)) 1
+      )end)
+    | _ => UConstr.iter collect e
+    end in
+  collect e; (st.(lets), st.(m), st.(n)).
+
+Ltac2 rec replace_consts (m : (constant, int) FMap.t) (n : int) (e : constr) : constr :=
+  match UConstr.kind e with
+  | UConstr.Constant c _ =>
+    match FMap.find_opt c m with
+    | Some i => UConstr.make (UConstr.Rel (Int.sub n i))
+    | None => e
+    end
+  | _ => UConstr.map_with_binders (fun n _ => Int.add n 1) (fun n c => replace_consts m n c) n e
+  end.
+
+Ltac2 let_lift_constants (filter : constant -> instance -> bool) (e : constr) : constr :=
+  let (lets, m, n) := collect_consts filter e in
+  snd (List.fold_left (fun (n, cont) (name_opt, typ, relevance, body) =>
+    let typ := replace_consts m n typ in
+    let body := replace_consts m n body in
+    let binder := Constr.Binder.unsafe_make name_opt relevance typ in
+    (Int.sub n 1, UConstr.make (UConstr.LetIn binder body cont))
+    ) (Int.sub n 1, replace_consts m n e) lets).
+
+Ltac2 let_lift_all_constants e := let_lift_constants (fun _ _ => true) e.
+
+Module Private_test.
+Definition n : nat. exact O. Defined.
+Ltac2 Eval let_lift_all_constants 'n.
+Definition A : Type := nat.
+Definition a : A. exact O. Defined.
+Ltac2 Eval let_lift_all_constants 'a.
+Definition B : Set := nat.
+Definition b : B. exact O. Defined.
+Ltac2 Eval let_lift_all_constants 'b.
+Definition base_val := 42.
+Definition t := nat.
+Definition m : t. exact O. Qed.
+Definition base_2  x  (y : nat) : nat := x + base_val * y.
+Ltac2 Eval let_lift_all_constants 'base_2.
+Definition base_2'  x  (y : t) : nat := x + base_val * y.
+Ltac2 Eval let_lift_all_constants 'base_2'.
+From Stdlib Require Import Zmod.
+Check (eq_refl : Z.div_eucl = ltac2:(let e := let_lift_all_constants 'Z.div_eucl in exact $e)).
+End Private_test.
